Prove the type safety

Term.v
@@ -1,7 +1,28 @@
-Require Import Arith Finite_sets_facts.
-Require Import Misc Types.
+Require Import Types.
+Require Import Autosubst.Autosubst.
 
-Inductive trm : Set :=
-  | trm_var (n : nat)
-  | trm_abs (t : trm)
+Inductive trm :=
+  | trm_var (n : var)
+  | trm_abs (t : { bind trm })
   | trm_app (t1 t2 : trm).
+
+Instance Ids_trm : Ids trm. derive. Defined.
+Instance Rename_trm : Rename trm. derive. Defined.
+Instance Subst_trm : Subst trm. derive. Defined.
+Instance SubstLemmas_trm : SubstLemmas trm. derive. Qed.
+
+Inductive value : trm -> Prop := val_abs t : value (trm_abs t).
+
+Inductive cbv : trm -> trm -> Prop :=
+  | cbv_appabs t11 v2 :
+      value v2 ->
+      cbv (trm_app (trm_abs t11) v2) (t11.[v2/])
+  | cbv_appl t1 t1' t2 :
+      cbv t1 t1' ->
+      cbv (trm_app t1 t2) (trm_app t1' t2)
+  | cbv_appr v1 t2 t2' :
+      value v1 ->
+      cbv t2 t2' ->
+      cbv (trm_app v1 t2) (trm_app v1 t2').
+
+Hint Constructors value cbv.
