TypeSafety.v
@@ -1,0 +1,66 @@
+Require Import List Relations.
+Require Import Types Term Typing.
+Require Import Autosubst.Autosubst.
+
+Lemma typed_rename G t T :
+  typed G t T ->
+  forall G' r,
+  (forall x T, nth_error G x = Some T -> nth_error G' (r x) = Some T) ->
+  typed G' (rename r t) T.
+Proof.
+  induction 1; simpl; eauto.
+  intros ? ? Hren. constructor. apply IHtyped.
+  intros [ ]; eauto.
+Qed.
+
+Lemma typed_subst G t T :
+  typed G t T ->
+  forall s G',
+  (forall x T, nth_error G x = Some T -> typed G' (s x) T) ->
+  typed G' (t.[s]) T.
+Proof.
+  induction 1; simpl; eauto.
+  intros ? ? Hs. constructor. apply IHtyped.
+  unfold up. intros [ ]; simpl; inversion 1; eauto.
+  apply typed_rename with (G := G'); eauto.
+Qed.
+
+Lemma subject_reduction t t' :
+  cbv t t' ->
+  forall G T, typed G t T ->
+  typed G t' T.
+Proof.
+  induction 1; inversion 1; subst; eauto.
+  inversion H4. subst.
+  apply typed_subst with (G := T1 :: G); eauto.
+  intros []; simpl; inversion 1; subst; eauto.
+Qed.
+
+Lemma normal_arrow v T1 T2 :
+  value v ->
+  typed nil v (typ_arrow T1 T2) ->
+  exists t, v = trm_abs t.
+Proof. inversion 1. eauto. Qed.
+
+Lemma progress G t T :
+  typed G t T ->
+  G = nil ->
+  value t \/ exists t', cbv t t'.
+Proof.
+  induction 1; intros; subst; eauto.
+  - destruct x; inversion H.
+  - destruct IHtyped1 as [ | [ ] ]; eauto.
+    edestruct normal_arrow; eauto. subst.
+    destruct IHtyped2 as [ | [ ] ]; eauto.
+Qed.
+
+Theorem type_safety t t' T :
+  typed nil t T ->
+  clos_refl_trans_1n _ cbv t t' ->
+  value t' \/ exists t'', cbv t' t''.
+Proof.
+  induction 2.
+  - eapply progress; eauto.
+  - apply IHclos_refl_trans_1n.
+    eapply subject_reduction; eauto.
+Qed.
